ancestor_context 에 ANil일 경우를 추가하고, walk_as_node 를 재작성

src/study/Nemonuri.Study.CSharpSyntaxRewriter2.Modifier2/Nemonuri.StratifiedNodes.AncestorContexts.Types.fst
@@ -9,7 +9,8 @@ module Id = Nemonuri.StratifiedNodes.Indexes
 //--- type definition ---
 
 type ancestor_context (t:eqtype) = 
-| AContext :
+| ANil: ancestor_context t
+| ACons:
   (ancestors: C.ancestor_list t) ->
   (indexes:list nat{Id.have_indexes ancestors indexes}) ->
   ancestor_context t
